added sign-magnitude (somewhat clunky) encoding; added talk slides

tools/splat/doc/may.2019/demo.ml
@@ -1,0 +1,88 @@
+(* use "provers.ml"; open provers;  *)
+
+val _ = new_theory "gps";
+
+val _ =
+ Hol_datatype
+   `gps = <| lat:  int ;
+             lon : int ;
+             alt : int |>`;
+
+val good_gps_def =
+  Define
+    `good_gps recd <=>
+         -90 <= recd.lat /\ recd.lat <= 90 /\
+         -180 <= recd.lon /\ recd.lon <= 180 /\
+         0 <= recd.alt /\ recd.alt <= 17999`;
+
+(*---------------------------------------------------------------------------*)
+(* Encode/decode gps elts                                                    *)
+(*---------------------------------------------------------------------------*)
+
+val encode_def =
+    Define
+    `encode recd =
+       CONCAT [encZ 1 recd.lat;
+               encZ 1 recd.lon;
+               encZ 2 recd.alt]`;
+
+(*---------------------------------------------------------------------------*)
+(* Note that decZ is total.                                                  *)
+(*---------------------------------------------------------------------------*)
+
+val decode_def =
+ Define
+  `decode s =
+    case s
+     of [a;b;c;d;e;f;g] =>
+        SOME <| lat := decZ [a;b];
+                lon := decZ [c;d];
+                alt := decZ [e;f;g] |>
+      | otherwise => NONE`;
+
+(*---------------------------------------------------------------------------*)
+(* Round trip theorem                                                        *)
+(*---------------------------------------------------------------------------*)
+
+Theorem decode_encode :
+  !m. good_gps m ==> (decode (encode m) = SOME m)
+Proof
+  ROUND_TRIP_TAC (encode_def, decode_def,good_gps_def)
+QED
+
+(*---------------------------------------------------------------------------*)
+(* Regexp expressing the interval constraints                                *)
+(*---------------------------------------------------------------------------*)
+
+val gps_regexp =
+    Regexp_Match.normalize
+        (Regexp_Type.fromQuote `\i{~90,90}\i{~180,180}\i{0,17999}`);
+
+val gps_regexp_term = regexpSyntax.regexp_to_term gps_regexp;
+
+(*---------------------------------------------------------------------------*)
+(* Compile regexp to a DFA                                                   *)
+(*---------------------------------------------------------------------------*)
+
+regexpLib.matcher regexpLib.SML gps_regexp;
+
+
+(*---------------------------------------------------------------------------*)
+(* Correctness theorem                                                       *)
+(*---------------------------------------------------------------------------*)
+
+Theorem AGREE_ENCODE_THM :
+  !m. good_gps m <=> encode(m) IN regexp_lang ^gps_regexp_term
+Proof
+  AGREE_ENCODE_TAC (encode_def, decode_def, good_gps_def)
+QED
+
+(*---------------------------------------------------------------------------*)
+(* Another correctness theorem                                               *)
+(*---------------------------------------------------------------------------*)
+
+Theorem AGREE_DECODE_THM :
+ !s. s IN regexp_lang ^gps_regexp_term ==> good_gps (THE (decode s))
+Proof
+  AGREE_DECODE_TAC (encode_def, decode_def, AGREE_ENCODE_THM)
+QED
