tools/splat/doc/may.2019/provers.sml
@@ -1,0 +1,497 @@
+open HolKernel Parse boolLib bossLib splatLib intLib;
+
+open arithmeticTheory listTheory stringTheory pred_setLib
+     FormalLangTheory charsetTheory regexpTheory regexpLib
+     numposrepTheory splatTheory;
+
+val int_ss = intSimps.int_ss;
+
+(*---------------------------------------------------------------------------*)
+(* Boilerplate prelude stuff                                                 *)
+(*---------------------------------------------------------------------------*)
+
+val _ = numLib.prefer_num();
+
+val _ = overload_on ("++",``list$APPEND``);
+
+infix byA;
+val op byA = BasicProvers.byA;
+
+val qpat_k_assum = Lib.C qpat_x_assum kall_tac;
+val allhyp_mp_tac = rpt (pop_assum mp_tac);
+val allhyp_kill_tac = rpt (pop_assum kall_tac);
+fun qpat_keeponly_assum qpat = qpat_x_assum qpat mp_tac >> allhyp_kill_tac
+
+fun qspec q th = th |> Q.SPEC q
+fun qspec_arith q th = qspec q th |> SIMP_RULE arith_ss [];
+
+val var_eq_tac = rpt BasicProvers.VAR_EQ_TAC;
+
+val decide = bossLib.DECIDE;
+val qdecide = decide o Parse.Term;
+
+val ERR = mk_HOL_ERR "DEMO";
+
+val regexp_lang_cat = el 2 (CONJUNCTS regexp_lang_def);
+val regexp_lang_or = last (CONJUNCTS regexp_lang_def);
+
+(*---------------------------------------------------------------------------*)
+(* Useful regexp rewrites                                                    *)
+(*---------------------------------------------------------------------------*)
+
+val in_chset_cat = Q.prove
+(`!s cs r.
+     s IN regexp_lang (Cat (Chset cs) r)
+       <=>
+     ?c t. (s = STRING c t) /\
+           (STRING c "") IN regexp_lang (Chset cs) /\ t IN regexp_lang r`,
+ rw_tac (list_ss ++ pred_setLib.PRED_SET_ss)
+        [regexp_lang_def,EQ_IMP_THM,IN_dot]
+ >> metis_tac [STRCAT_EQNS])
+
+val in_chset = Q.prove
+(`!n cs s L.
+     STRING c s IN regexp_lang (Chset cs) dot L
+       <=>
+     (STRING c "") IN regexp_lang (Chset cs) /\ s IN L`,
+ rw_tac (list_ss ++ pred_setLib.PRED_SET_ss)
+        [regexp_lang_def,EQ_IMP_THM,IN_dot]
+ >> full_simp_tac list_ss []
+ >> var_eq_tac
+ >- metis_tac[]
+ >- (qexists_tac `STRING (CHR c') ""`
+     >> qexists_tac `s`
+     >> rw_tac list_ss []
+     >> metis_tac[])
+);
+
+val not_in_chset = Q.prove
+(`!cs. "" NOTIN regexp_lang (Chset cs)`,
+ rw_tac (list_ss ++ pred_setLib.PRED_SET_ss)
+        [regexp_lang_def,EQ_IMP_THM,IN_dot]);
+
+Theorem ORD_EQ :
+ !c n. (ORD c = n) <=> ((CHR n = c) /\ n < 256)
+Proof
+  metis_tac [CHR_ORD,ORD_CHR_RWT,ORD_BOUND]
+QED
+
+val two_leq_length = Q.prove
+(`!L. (2 <= LENGTH L) <=> ?a b t. L = a::b::t`,
+  Cases_on `L` >> rw_tac list_ss [] >>
+  Cases_on `t` >> rw_tac list_ss []);
+
+val APPEND_EQ_CONS_ALT = Q.prove
+(`!l1 l2 h t.
+  ((l1 ++ l2 = h::t) <=> ((l1 = []) /\ (l2 = h::t)) \/ (∃lt. (l1 = h::lt) ∧ (t = lt ⧺ l2)))
+  /\
+  ((h::t = l1 ++ l2) <=> ((l1 = []) ∧ (l2 = h::t)) ∨ (∃lt. (l1 = h::lt) ∧ (t = lt ⧺ l2)))`,
+ metis_tac [APPEND_EQ_CONS]);
+
+val len_lem = Q.prove
+(`!A B C.
+   (2 <= LENGTH A) /\ (2 <= LENGTH B) /\ (3 <= LENGTH C) /\
+(A ++ B ++ C = [c1;c2;c3;c4;c5;c6;c7])
+  ==>
+  (A = [c1;c2]) /\ (B = [c3;c4]) /\ (C = [c5;c6;c7])`,
+ rw_tac list_ss [APPEND_EQ_CONS_ALT,two_leq_length]
+ >> full_simp_tac list_ss [APPEND_EQ_CONS_ALT]);
+
+(* Needs some thought *)
+(*
+Theorem enc_dec :
+ !s. enc (LENGTH s) (dec s) = s
+Proof
+rw_tac list_ss [dec_def, l2n_def,ord_mod_256,ORD_CHR_RWT]
+QED
+*)
+
+
+Theorem decZ_eqns :
+  (!s s'. decZ (STRING #"+" s') = int_of_num (dec s')) /\
+  (!s s'. decZ (STRING #"-" s') = -(int_of_num (dec s')))
+Proof
+rw_tac list_ss [decZ_def,CHR_11]
+QED
+
+Theorem strlen_encZ :
+  !w i. STRLEN (encZ w i) = 1 + STRLEN (enc w (Num(ABS i)))
+Proof
+rw_tac list_ss [encZ_def]
+QED
+
+Theorem dec_char :
+  !c. dec [c] = ORD c
+Proof
+ rw_tac list_ss [dec_def,l2n_def,ord_mod_256]
+QED
+
+val [encz1,encz2,encz3,encz4,encz8] = CONJUNCTS encZ_bytes;
+
+val [enc1,enc2,enc3,enc4,enc5,enc6,enc7,encz8]
+    = CONJUNCTS (SIMP_RULE arith_ss [] enc_bytes);
+
+(*---------------------------------------------------------------------------*)
+(* Reduce charsets to constraints                                            *)
+(*---------------------------------------------------------------------------*)
+
+fun regexp_elts r =
+   Regexp_Type.charset_elts
+     (regexpSyntax.term_to_charset r);
+
+fun charset_intervals r =
+  let fun endpoints list = (IntInf.toInt (hd list),IntInf.toInt (last list))
+  in map endpoints
+      (Interval.intervals
+         (map (IntInf.fromInt o Char.ord) (regexp_elts r)))
+  end
+
+fun CHECK_SPEC_TAC (t1,t2) (asl,c) =
+  (if can(find_term (aconv t1)) c
+    then SPEC_TAC (t1,t2)
+    else NO_TAC) (asl,c)
+
+fun GEVAL_TAC (asl,c) =
+    (if null(free_vars c) then EVAL_TAC else NO_TAC) (asl,c);
+
+fun const_bound tm =
+ let open numSyntax
+ in (is_less tm orelse is_leq tm)
+    andalso
+    is_numeral (rand tm)
+ end
+
+val ordered_pop_tac =
+ rpt (PRED_ASSUM (not o const_bound) mp_tac)
+  >> PRED_ASSUM const_bound mp_tac;
+
+val prover =
+ let open numSyntax stringSyntax
+     val cvar = mk_var("c",num)
+     val nvar = mk_var("n",num)
+     val ordtm = mk_ord(mk_var("c",char_ty))
+ in
+    rw_tac (list_ss ++ pred_setLib.PRED_SET_ss)
+      [pred_setTheory.EXTENSION, regexpTheory.regexp_lang_def,
+       charsetTheory.charset_mem_def, charsetTheory.alphabet_size_def,
+       EQ_IMP_THM,strlen_eq,LE_LT1]
+    >> full_simp_tac list_ss [dec_char,ORD_CHR_RWT]
+    >> TRY (qexists_tac `ORD c` >> rw_tac list_ss [CHR_ORD])
+    >> (GEVAL_TAC ORELSE
+         (ordered_pop_tac
+           >> (CHECK_SPEC_TAC (cvar,nvar) ORELSE
+               CHECK_SPEC_TAC (ordtm,nvar))
+           >> REPEAT (CONV_TAC (numLib.BOUNDED_FORALL_CONV EVAL))
+           >> gen_tac >> ACCEPT_TAC TRUTH))
+ end
+
+(*---------------------------------------------------------------------------*)
+(* Takes a term of the form                                                  *)
+(*                                                                           *)
+(*  s IN regexp_lang (Chset (Charset a b c d))                               *)
+(*                                                                           *)
+(* and returns                                                               *)
+(*                                                                           *)
+(* |- s IN regexp_lang (Chset (Charset a b c d)) <=>                         *)
+(*    STRLEN s = 1 /\ lo <= dec s <= hi                                      *)
+(*                                                                           *)
+(* where lo and hi are the interval endpoints. If lo = 0 then it is omitted. *)
+(* If lo=hi then we just have (dec s = lo)                                   *)
+(*---------------------------------------------------------------------------*)
+
+fun pure_in_charset_conv tm =
+ let open regexpSyntax stringSyntax pred_setSyntax numSyntax
+     val (s,rlang) = dest_in tm
+     val reg = dest_chset(dest_regexp_lang rlang)
+     val ivls = charset_intervals reg
+     fun ivl_to_prop (lo,hi) =
+         if lo = hi then
+            ``dec ^s = ^(term_of_int lo)``
+         else
+         if lo = 0 then
+            ``dec ^s < ^(term_of_int(hi + 1))``
+         else
+            ``^(term_of_int lo) <= dec ^s /\ dec ^s <= ^(term_of_int hi)``
+     val slen = ``STRLEN ^s = 1``
+     val property = mk_eq(tm, mk_conj(slen,list_mk_disj (map ivl_to_prop ivls)))
+ in
+    prove(property,prover)
+ end
+
+
+fun dest_in_chset tm =
+ let open regexpSyntax
+     val (s,rlang) = pred_setSyntax.dest_in tm
+ in
+     dest_chset(dest_regexp_lang rlang)
+ end
+
+(*---------------------------------------------------------------------------*)
+(* Make a memo-izing version of the charset-to-interval conv.                *)
+(*---------------------------------------------------------------------------*)
+
+val in_charset_conv =
+ let val conv =
+      Conv.memoize
+        (Lib.total dest_in_chset)
+        (Redblackmap.fromList Term.compare [])
+(*
+          (map (fn th => (dest_in_chset(lhs(concl th)),th))
+               charset_interval_lems))
+*)
+       (K true)
+       (ERR "in_charset_conv (memoized)" "")
+       pure_in_charset_conv
+ in fn tm =>
+      let val thm = conv tm
+          val left = lhs(concl thm)
+      in
+        if aconv tm left then
+          thm
+        else
+          INST (fst (match_term left tm)) thm
+      end
+ end;
+
+(*---------------------------------------------------------------------------*)
+(* Construct a simplification set from the memoized conversion.              *)
+(*---------------------------------------------------------------------------*)
+
+val in_charset_conv_ss =
+ let val csvar = mk_var("cs",regexpSyntax.charset_ty)
+     val svar = mk_var("s",stringSyntax.string_ty)
+     val regexp_chset_pat = ``^svar IN regexp$regexp_lang ^(regexpSyntax.mk_chset csvar)``
+ in
+  simpLib.std_conv_ss
+    {name = "in_charset_conv",
+     conv = in_charset_conv,
+     pats = [regexp_chset_pat]}
+ end
+
+fun ROUND_TRIP_TAC (encode_def, decode_def, good_gps_def) =
+ rw_tac list_ss [decode_def, encode_def, list_case_eq, PULL_EXISTS,good_gps_def,
+                 fetch "-" "gps_component_equality"]
+  >> `-256 < m.lat /\ m.lat < 256 /\
+      -256 < m.lon /\ m.lon < 256 /\
+      -65536 < m.alt /\ m.alt < 65536` by intLib.ARITH_TAC
+  >> imp_res_tac encz1
+  >> imp_res_tac encz2
+  >> rw_tac (srw_ss()) []
+  >> metis_tac [decz_encz]
+;
+
+fun enforce tac gl = (tac gl handle HOL_ERR _ => cheat gl);
+
+fun AGREE_ENCODE_TAC (encode_def, decode_def, good_gps_def) =
+enforce
+(rw_tac list_ss [regexp_lang_cat,IN_dot,PULL_EXISTS,encode_def,EQ_IMP_THM]
+  >- (rw_tac (list_ss ++ in_charset_conv_ss)
+       [regexp_lang_cat,regexp_lang_or,LIST_UNION_def,IN_dot,strlen_eq,PULL_EXISTS,dec_char]
+     >> qexists_tac `encZ 1 m.lat`
+     >> qexists_tac `encZ 1 m.lon`
+     >> qexists_tac `enc 2 (Num (ABS m.alt))`
+     >> qexists_tac `#"+"`
+     >> simp_tac bool_ss [GSYM STRCAT_ASSOC,STRCAT_11]
+     >> full_simp_tac list_ss [good_gps_def]
+     >> rpt conj_tac
+        >- metis_tac [encZ_def]
+        >- (ntac 4 (pop_assum kall_tac)
+            >> Cases_on `m.lat < 0` THENL [disj2_tac, disj1_tac]
+            >> `Num(ABS m.lat) < 256` by intLib.ARITH_TAC
+            >> rw_tac int_ss [encZ_def,enc_bytes,ORD_CHR_RWT]
+            >> intLib.ARITH_TAC)
+        >- (ntac 2 (pop_assum kall_tac)
+            >> ntac 2 (pop_assum mp_tac)
+            >> ntac 2 (pop_assum kall_tac)
+            >> rpt strip_tac
+            >> Cases_on `m.lon < 0` THENL [disj2_tac, disj1_tac]
+            >> `Num(ABS m.lon) < 256` by intLib.ARITH_TAC
+            >> rw_tac int_ss [encZ_def,enc_bytes,ORD_CHR_RWT]
+            >> intLib.ARITH_TAC)
+        >- EVAL_TAC
+        >- (ntac 2 (pop_assum mp_tac)
+            >> rpt (pop_assum kall_tac)
+            >> rpt strip_tac
+            >> `m.alt >= 256 * 70 \/ m.alt < 256 * 70`
+                  by intLib.ARITH_TAC
+            THENL [disj1_tac,disj2_tac]
+            >- (`Num(ABS m.alt) < 65536` by intLib.ARITH_TAC
+                >> rw_tac int_ss [enc_bytes,ORD_CHR_RWT]
+                >> intLib.ARITH_TAC)
+            >- (Cases_on `m.alt < 256` THENL [disj1_tac,disj2_tac]
+                >- (`Num(ABS m.alt) < 256` by intLib.ARITH_TAC
+                     >> rw_tac int_ss [enc_bytes,ORD_CHR_RWT]
+                     >> intLib.ARITH_TAC)
+                >- (`Num(ABS m.alt) < 65536` by intLib.ARITH_TAC
+                     >> rw_tac int_ss [enc_bytes,ORD_CHR_RWT]
+                     >> intLib.ARITH_TAC)))
+    )
+ (* second part *)
+ >- (`2 <= LENGTH (encZ 1 m.lat) /\ 2 <= LENGTH (encZ 1 m.lon) /\ 3 <= LENGTH (encZ 2 m.alt)`
+        byA (rw_tac list_ss [strlen_encZ]
+             >> metis_tac [lower_enc, qdecide `2n = 1 + 1`, qdecide `3n = 2 + 1`,
+                           arithmeticTheory.LE_ADD_RCANCEL])
+     >> full_simp_tac (list_ss ++ in_charset_conv_ss)
+              [regexp_lang_cat,regexp_lang_or,LIST_UNION_def,
+               IN_dot,strlen_eq,PULL_EXISTS,dec_char]
+     >> rw_tac list_ss []
+     >> full_simp_tac list_ss [dec_char,ORD_EQ]
+     >> rw_tac list_ss []
+     >> `?c c1 c2 c3 c4 c5 c6.
+          (encZ 1 m.lat = [c;c1]) /\ (encZ 1 m.lon = [c2;c3]) /\ (encZ 2 m.alt = [c4;c5;c6])`
+            by metis_tac [len_lem]
+     >> full_simp_tac list_ss [encZ_def]
+     >> BasicProvers.NORM_TAC list_ss [CHR_11]
+     >> asm_simp_tac list_ss [good_gps_def]
+     >> `(m.lat = decZ (encZ 1 m.lat)) /\
+         (m.lon = decZ (encZ 1 m.lon)) /\
+         (m.alt = decZ (encZ 1 m.alt))` by metis_tac [decz_encz]
+     >> ntac 3 (pop_assum SUBST1_TAC)
+     >> asm_simp_tac bool_ss [encZ_def]
+     >> asm_simp_tac int_ss [decZ_eqns,dec_char,dec_enc]
+     >> qpat_x_assum `enc 2 _ = _` (mp_tac o AP_TERM ``dec``)
+     >> rw_tac list_ss [dec_enc, dec_def, l2n_def,ord_mod_256,ORD_CHR_RWT]
+    )
+)
+;
+
+fun AGREE_DECODE_TAC (encode_def, decode_def, AGREE_ENCODE_THM) =
+enforce
+ (rw_tac std_ss [AGREE_ENCODE_THM]
+  >> full_simp_tac (list_ss ++ in_charset_conv_ss)
+       [regexp_lang_cat,regexp_lang_or,LIST_UNION_def,IN_dot,strlen_eq,PULL_EXISTS,dec_char,ORD_EQ]
+  >> rw_tac list_ss [decode_def,decZ_eqns,dec_char]
+  >> rw_tac (srw_ss()) [encode_def]
+  >- (qexists_tac `[#"+"; c']`
+      >> qexists_tac `[#"+"; c'']`
+      >> qexists_tac `[c;#"F"]`
+      >> rw_tac int_ss [encZ_def,enc_bytes,CHR_ORD]
+      >> rw_tac std_ss [STRCAT_EQNS]
+      >> rw_tac list_ss [dec_def, l2n_def,ord_mod_256,ORD_CHR_RWT]
+      >> rw_tac int_ss [enc_bytes]
+         >- rw_tac list_ss [Once (GSYM MOD_PLUS),CHR_ORD]
+         >- rw_tac list_ss [ADD_DIV_RWT,LESS_DIV_EQ_ZERO])
+
+  >- (qexists_tac `[#"+"; c']`
+      >> qexists_tac `[#"+"; c'']`
+      >> qexists_tac `[c;#"\^@"]`
+      >> rw_tac int_ss [encZ_def,enc_bytes,CHR_ORD]
+      >> rw_tac std_ss [STRCAT_EQNS]
+      >> rw_tac list_ss [dec_def, l2n_def,ord_mod_256,ORD_CHR_RWT]
+      >> rw_tac int_ss [enc_bytes]
+         >- rw_tac list_ss [Once (GSYM MOD_PLUS),CHR_ORD]
+         >- rw_tac list_ss [ADD_DIV_RWT,LESS_DIV_EQ_ZERO])
+
+  >- (qexists_tac `[#"+"; c']`
+      >> qexists_tac `[#"+"; c'']`
+      >> qexists_tac `[c;c''']`
+      >> rw_tac int_ss [encZ_def,enc_bytes,CHR_ORD]
+      >> rw_tac std_ss [STRCAT_EQNS]
+      >> rw_tac list_ss [dec_def, l2n_def,ord_mod_256,ORD_CHR_RWT]
+      >> rw_tac int_ss [enc_bytes]
+         >- (rw_tac bool_ss [Once ADD_SYM,Once MULT_SYM]
+              >> rw_tac list_ss [MOD_MULT,CHR_ORD])
+         >- (rw_tac (srw_ss()) [ADD_DIV_RWT,LESS_DIV_EQ_ZERO]
+              >> rw_tac bool_ss [Once MULT_SYM]
+              >> rw_tac std_ss [MULT_DIV,ord_mod_256,CHR_ORD]))
+
+  >- (qexists_tac `[#"+"; c']`
+      >> qexists_tac `[#"-"; c'']`
+      >> qexists_tac `[c;#"F"]`
+      >> rw_tac int_ss [encZ_def,enc_bytes,CHR_ORD]
+      >> rw_tac std_ss [STRCAT_EQNS]
+      >> rw_tac list_ss [dec_def, l2n_def,ord_mod_256,ORD_CHR_RWT]
+      >> rw_tac int_ss [enc_bytes]
+         >- rw_tac list_ss [Once (GSYM MOD_PLUS),CHR_ORD]
+         >- rw_tac list_ss [ADD_DIV_RWT,LESS_DIV_EQ_ZERO])
+
+  >- (qexists_tac `[#"+"; c']`
+      >> qexists_tac `[#"-"; c'']`
+      >> qexists_tac `[c;#"\^@"]`
+      >> rw_tac int_ss [encZ_def,enc_bytes,CHR_ORD]
+      >> rw_tac std_ss [STRCAT_EQNS]
+      >> rw_tac list_ss [dec_def, l2n_def,ord_mod_256,ORD_CHR_RWT]
+      >> rw_tac int_ss [enc_bytes]
+         >- rw_tac list_ss [Once (GSYM MOD_PLUS),CHR_ORD]
+         >- rw_tac list_ss [ADD_DIV_RWT,LESS_DIV_EQ_ZERO])
+
+  >- (qexists_tac `[#"+"; c']`
+      >> qexists_tac `[#"-"; c'']`
+      >> qexists_tac `[c;c''']`
+      >> rw_tac int_ss [encZ_def,enc_bytes,CHR_ORD]
+      >> rw_tac std_ss [STRCAT_EQNS]
+      >> rw_tac list_ss [dec_def, l2n_def,ord_mod_256,ORD_CHR_RWT]
+      >> rw_tac int_ss [enc_bytes]
+         >- (rw_tac bool_ss [Once ADD_SYM,Once MULT_SYM]
+              >> rw_tac list_ss [MOD_MULT,CHR_ORD])
+         >- (rw_tac (srw_ss()) [ADD_DIV_RWT,LESS_DIV_EQ_ZERO]
+              >> rw_tac bool_ss [Once MULT_SYM]
+              >> rw_tac std_ss [MULT_DIV,ord_mod_256,CHR_ORD]))
+
+  >- (qexists_tac `[#"-"; c']`
+      >> qexists_tac `[#"+"; c'']`
+      >> qexists_tac `[c;#"F"]`
+      >> rw_tac int_ss [encZ_def,enc_bytes,CHR_ORD]
+      >> rw_tac std_ss [STRCAT_EQNS]
+      >> rw_tac list_ss [dec_def, l2n_def,ord_mod_256,ORD_CHR_RWT]
+      >> rw_tac int_ss [enc_bytes]
+         >- rw_tac list_ss [Once (GSYM MOD_PLUS),CHR_ORD]
+         >- rw_tac list_ss [ADD_DIV_RWT,LESS_DIV_EQ_ZERO])
+
+  >- (qexists_tac `[#"-"; c']`
+      >> qexists_tac `[#"+"; c'']`
+      >> qexists_tac `[c;#"\^@"]`
+      >> rw_tac int_ss [encZ_def,enc_bytes,CHR_ORD]
+      >> rw_tac std_ss [STRCAT_EQNS]
+      >> rw_tac list_ss [dec_def, l2n_def,ord_mod_256,ORD_CHR_RWT]
+      >> rw_tac int_ss [enc_bytes]
+         >- rw_tac list_ss [Once (GSYM MOD_PLUS),CHR_ORD]
+         >- rw_tac list_ss [ADD_DIV_RWT,LESS_DIV_EQ_ZERO])
+
+  >- (qexists_tac `[#"-"; c']`
+      >> qexists_tac `[#"+"; c'']`
+      >> qexists_tac `[c;c''']`
+      >> rw_tac int_ss [encZ_def,enc_bytes,CHR_ORD]
+      >> rw_tac std_ss [STRCAT_EQNS]
+      >> rw_tac list_ss [dec_def, l2n_def,ord_mod_256,ORD_CHR_RWT]
+      >> rw_tac int_ss [enc_bytes]
+         >- (rw_tac bool_ss [Once ADD_SYM,Once MULT_SYM]
+              >> rw_tac list_ss [MOD_MULT,CHR_ORD])
+         >- (rw_tac (srw_ss()) [ADD_DIV_RWT,LESS_DIV_EQ_ZERO]
+              >> rw_tac bool_ss [Once MULT_SYM]
+              >> rw_tac std_ss [MULT_DIV,ord_mod_256,CHR_ORD]))
+
+  >- (qexists_tac `[#"-"; c']`
+      >> qexists_tac `[#"-"; c'']`
+      >> qexists_tac `[c;#"F"]`
+      >> rw_tac int_ss [encZ_def,enc_bytes,CHR_ORD]
+      >> rw_tac std_ss [STRCAT_EQNS]
+      >> rw_tac list_ss [dec_def, l2n_def,ord_mod_256,ORD_CHR_RWT]
+      >> rw_tac int_ss [enc_bytes]
+         >- rw_tac list_ss [Once (GSYM MOD_PLUS),CHR_ORD]
+         >- rw_tac list_ss [ADD_DIV_RWT,LESS_DIV_EQ_ZERO])
+
+  >- (qexists_tac `[#"-"; c']`
+      >> qexists_tac `[#"-"; c'']`
+      >> qexists_tac `[c;#"\^@"]`
+      >> rw_tac int_ss [encZ_def,enc_bytes,CHR_ORD]
+      >> rw_tac std_ss [STRCAT_EQNS]
+      >> rw_tac list_ss [dec_def, l2n_def,ord_mod_256,ORD_CHR_RWT]
+      >> rw_tac int_ss [enc_bytes]
+         >- rw_tac list_ss [Once (GSYM MOD_PLUS),CHR_ORD]
+         >- rw_tac list_ss [ADD_DIV_RWT,LESS_DIV_EQ_ZERO])
+
+  >- (qexists_tac `[#"-"; c']`
+      >> qexists_tac `[#"-"; c'']`
+      >> qexists_tac `[c;c''']`
+      >> rw_tac int_ss [encZ_def,enc_bytes,CHR_ORD]
+      >> rw_tac std_ss [STRCAT_EQNS]
+      >> rw_tac list_ss [dec_def, l2n_def,ord_mod_256,ORD_CHR_RWT]
+      >> rw_tac int_ss [enc_bytes]
+         >- (rw_tac bool_ss [Once ADD_SYM,Once MULT_SYM]
+              >> rw_tac list_ss [MOD_MULT,CHR_ORD])
+         >- (rw_tac (srw_ss()) [ADD_DIV_RWT,LESS_DIV_EQ_ZERO]
+              >> rw_tac bool_ss [Once MULT_SYM]
+              >> rw_tac std_ss [MULT_DIV,ord_mod_256,CHR_ORD]))
+);
+
